wip

steel/Veritas.Formats.fsti
@@ -13,12 +13,27 @@ val serialize_value: v:value -> dst: A.array U8.t { A.length dst == U32.v (seria
     (A.varray dst)
     (fun _ -> A.varray dst)
 
-val extract_log_entry_from (len: U32.t) (buf: A.array U8.t { A.length buf == U32.v len }) (pos: A.array (x: U32.t { U32.v x <= U32.v len }) { A.length pos == 1 })
-  : SteelT (option vlog_entry)
-    (A.varray buf `star` A.varray pos)
-    (fun _ -> A.varray buf `star` A.varray pos)
- (* /\
-            log at position h0.pos contains a vali repr of v *)
+module R = Steel.Reference
+
+let bounded_u32 (l:nat) = x:U32.t { U32.v x <= l }
+
+let larray t (l:U32.t) = a:A.array t { A.length a == U32.v l }
+
+val valid_entry (s:Seq.seq U8.t) (from:nat) (to:nat) (e:vlog_entry) : prop
+
+val extract_log_entry_from (len: U32.t)
+                           (buf: larray U8.t len)
+                           (pos: R.ref (bounded_u32 (U32.v len)))
+  : Steel (option vlog_entry)
+    (A.varray buf `star` R.vptr pos)
+    (fun _ -> A.varray buf `star` R.vptr pos)
+    (requires fun _ -> True)
+    (ensures fun h0 x h1 ->
+      A.asel buf h0 == A.asel buf h1 /\
+      (match x with
+       | None -> True
+       | Some e ->
+         valid_entry (A.asel buf h0) (U32.v (R.sel pos h0)) (U32.v (R.sel pos h1)) e))
 
 val serialize_stamped_record
   (dst: A.array U8.t { 184 <= A.length dst })
