steel/Veritas.Steel.Log.fst
@@ -1,0 +1,363 @@
+module Veritas.Steel.Log
+module T = Veritas.Formats.Types
+module A = Steel.Array
+module U8 = FStar.UInt8
+module U32 = FStar.UInt32
+module EP = Veritas.Formats
+module R = Steel.Reference
+
+let bytes_repr (l:nat) = Ghost.erased (Seq.lseq U8.t l)
+
+let rec parsed_raw (s:Seq.seq U8.t) (r: repr)
+  : Tot Type
+    (decreases (Seq.length s))
+  = if Seq.length r = 0 then True
+    else (
+      exists (to:nat{0 < to /\ to <= Seq.length s}).
+           EP.valid_entry s 0 to (Seq.head r) /\
+           parsed_raw (Seq.slice s to (Seq.length s)) (Seq.tail r)
+    )
+
+let parsed_raw_until
+      (#len:nat)
+      (pos:EP.bounded_u32 len)
+      (s:bytes_repr len)
+      (r:repr)
+  = parsed_raw (Seq.slice s 0 (U32.v pos)) r
+
+let extend_parsed_raw_util
+      (#len:nat)
+      (pos:EP.bounded_u32 len)
+      (s:bytes_repr len)
+      (r:repr)
+      (pos':EP.bounded_u32 len)
+      (e:T.vlog_entry)
+  : Lemma
+    (requires
+      parsed_raw_until pos s r /\
+      EP.valid_entry s (U32.v pos) (U32.v pos') e)
+    (ensures
+      parsed_raw_until pos' s (snoc_log r e))
+  = admit()
+
+let parsed s r = parsed_raw s (FStar.Ghost.reveal r)
+
+noeq
+type log = {
+  len   : U32.t;
+  arr   : EP.larray U8.t len;
+  pos   : R.ref (EP.bounded_u32 (U32.v len));
+  ghost : R.ghost_ref (Seq.seq T.vlog_entry)
+}
+
+let log_len l = l.len
+let log_array l = l.arr
+
+let log_length l = U32.v (log_len l)
+
+let contents #t (a:A.array t) = A.contents t (A.length a)
+
+assume
+val varray_pts_to (#t:_) (a:A.array t) (bs:Ghost.erased (contents a)) : vprop
+
+let raw_log_pts_to (a:A.array U8.t) (bs:bytes_repr (A.length a)) =
+  varray_pts_to a bs
+
+module AT = Steel.Effect.Atomic
+
+assume
+val intro_varray_pts_to (#t:_)
+                        (#opened:inames)
+                        (a:A.array t)
+  : AT.SteelGhost (Ghost.erased (contents a)) opened
+    (A.varray a)
+    (fun x -> varray_pts_to a x `star` emp)
+    (requires fun _ -> True)
+    (ensures fun h0 x h1 ->
+      Ghost.reveal x == A.asel a h0)
+
+assume
+val varray_pts_to_u8 (#len:_)
+                     (a:EP.larray U8.t len)
+                     (bs:bytes_repr (U32.v len))
+  : vprop
+
+assume
+val intro_varray_pts_to_u8 (#opened:inames)
+                           (#len: U32.t)
+                           (arr: EP.larray U8.t len)
+  : AT.SteelGhost (bytes_repr (U32.v len)) opened
+    (A.varray arr)
+    (fun x -> varray_pts_to_u8 arr x `star` emp)
+    (requires fun _ -> True)
+    (ensures fun h0 x h1 ->
+      Ghost.reveal x == A.asel arr h0)
+
+module Perm = Steel.FractionalPermission
+[@@__reduce__; __steel_reduce__]
+let log_with_parsed_prefix_raw
+       (len: U32.t)
+       (arr: EP.larray U8.t len)
+       (pos: R.ref (EP.bounded_u32 (U32.v len)))
+       (ghost: R.ghost_ref (Seq.seq T.vlog_entry))
+       (pos_val: EP.bounded_u32 (U32.v len))
+       (bs : bytes_repr (U32.v len))
+       (s  : repr)
+  : vprop
+  = R.pts_to pos Perm.full_perm pos_val `star`
+    varray_pts_to_u8 arr bs `star`
+    R.ghost_pts_to ghost Perm.full_perm s `star`
+    pure (parsed_raw_until pos_val bs s)
+
+let parsed_raw_until_empty (len:_)
+                           (pos:EP.bounded_u32 (U32.v len) { pos == 0ul })
+                           (s:bytes_repr (U32.v len))
+  : Lemma (parsed_raw_until pos s Seq.empty)
+  = admit()
+
+//[@@__reduce__; __steel_reduce__]
+let log_with_parsed_prefix (l:log) (s:repr)
+  = AT.h_exists (fun p ->
+    AT.h_exists (fun bs ->
+    log_with_parsed_prefix_raw l.len l.arr l.pos l.ghost p bs s))
+
+let coerce_bounded_u32 (l:log) (len:U32.t) (x:EP.bounded_u32 (U32.v len))
+  : Pure
+     (EP.bounded_u32 (U32.v l.len))
+     (requires l.len == len)
+     (fun _ -> True)
+  = x
+
+let coerce_bytes_repr (l:log) (len:U32.t) (x:bytes_repr (U32.v len))
+  : Pure
+     (bytes_repr (U32.v l.len))
+     (requires l.len == len)
+     (fun _ -> True)
+  = x
+
+let coerce_eq (#a:Type) (#t: a -> Type) (x:a) (y:a) (v:t x)
+  : Pure (t y)
+     (requires x==y)
+     (fun _ -> True)
+  = v
+
+//module T = FStar.Tactics
+let intro_log_with_parsed_prefix
+     (l:log)
+     (len:U32.t)
+     (arr:EP.larray U8.t len)
+     (pos:R.ref (EP.bounded_u32 (U32.v len)))
+     (ghost: R.ghost_ref (Seq.seq T.vlog_entry))
+     (pos_val: EP.bounded_u32 (U32.v len))
+     (bs : bytes_repr (U32.v len))
+     (s  : repr)
+     (_  : squash (l.len == len))
+ : Steel unit
+   (log_with_parsed_prefix_raw len arr pos ghost pos_val bs s)
+   (fun _ -> log_with_parsed_prefix l s)
+   (requires fun _ ->
+     l.len == len /\
+     l.arr == arr /\
+     l.pos == pos /\
+     l.ghost == ghost)
+   (ensures fun _ _ _ -> True)
+ = let h = AT.get () in
+   assert (l.len == len);
+   let pos_val' : EP.bounded_u32 (U32.v l.len) = coerce_bounded_u32 l len pos_val in
+   let bs' : bytes_repr (U32.v l.len) = coerce_bytes_repr l len bs in
+   assert_spinoff(log_with_parsed_prefix_raw len arr pos ghost pos_val bs s ==
+                  log_with_parsed_prefix_raw l.len l.arr l.pos l.ghost pos_val' bs' s);
+   AT.change_equal_slprop
+     (log_with_parsed_prefix_raw len arr pos ghost pos_val bs s)
+     (log_with_parsed_prefix_raw l.len l.arr l.pos l.ghost pos_val' bs' s);
+   AT.intro_exists bs'
+                   (fun bs' -> log_with_parsed_prefix_raw l.len l.arr l.pos l.ghost pos_val' bs' s);
+   AT.intro_exists pos_val'
+                   (fun pos_val' ->
+                     AT.h_exists
+                     (fun bs' -> log_with_parsed_prefix_raw l.len l.arr l.pos l.ghost pos_val' bs' s));
+   AT.return ()
+
+let initialize_log' (len:U32.t) (a:EP.larray U8.t len)
+  : Steel log
+    (A.varray a)
+    (fun l -> log_with_parsed_prefix l empty_log)
+    (requires fun _ ->
+      A.length a == U32.v len)
+    (ensures fun _ l _ ->
+      log_len l == len /\
+      log_array l == a)
+  = let pos = R.alloc_pt 0ul in
+    let ghost = R.ghost_alloc_pt (Ghost.hide Seq.empty) in
+    let contents = intro_varray_pts_to_u8 a in
+    parsed_raw_until_empty len 0ul contents;
+    AT.intro_pure (parsed_raw_until #(U32.v len) 0ul contents (Ghost.hide Seq.empty));
+    let log = {
+      len = len;
+      arr = a;
+      pos = pos;
+      ghost = ghost
+    } in
+    AT.slassert (log_with_parsed_prefix_raw len a pos ghost 0ul contents (Ghost.hide Seq.empty));
+    let s : squash (log.len == len) = () in
+    intro_log_with_parsed_prefix log len a pos ghost 0ul contents (Ghost.hide Seq.empty) s;
+    AT.return log
+
+let initialize_log len a = initialize_log' len a
+
+let parsed_log (l:log) (s:repr) : vprop =
+   pure (U32.v l.len == Seq.length s) `star`
+   R.ghost_pts_to l.ghost Perm.full_perm s
+
+let parsed_log_inv l s =
+  let open AT in
+  (U32.v l.len == Seq.length s) /\
+  (exists (i:iname). i >--> parsed_log l s)
+
+#push-options "--query_stats --log_queries"
+let dummy () = ()
+
+val read_next' (#s:repr) (l:log)
+  : Steel read_result
+    (log_with_parsed_prefix l s)
+    (read_next_provides s l)
+    (requires fun _ -> True)
+    (ensures fun _ o h1 ->
+      match o with
+      | Finished ->
+        //The entries we parsed is stable and fixed to s
+        parsed_log_inv l s /\
+        //and s is the parse of the contents of the array in state h1
+        parsed (array_sel (log_array l) (rmem_coerce h1)) s
+      | Parsed_with_maybe_more e -> True
+      | Failed pos _ -> U32.(pos <^ log_len l))
+#restart-solver
+#push-options "--ide_id_info_off"
+let elim_log_with_parsed_prefix
+     (l:log)
+     (s  : repr)
+ : SteelT (Ghost.erased (EP.bounded_u32 (U32.v l.len)) &
+           bytes_repr (U32.v l.len))
+   (log_with_parsed_prefix l s)
+   (fun r -> log_with_parsed_prefix_raw l.len l.arr l.pos l.ghost (fst r) (snd r) s)
+ = let p =
+       AT.witness_exists
+         #_ #_
+         #(fun (p:EP.bounded_u32 (U32.v l.len)) ->
+           AT.h_exists (fun bs -> log_with_parsed_prefix_raw l.len l.arr l.pos l.ghost p bs s))
+         ()
+   in
+   let bs = AT.witness_exists #_ #_
+     #(fun bs -> log_with_parsed_prefix_raw l.len l.arr l.pos l.ghost p bs s)
+     ()
+   in
+   AT.return (p, Ghost.reveal bs)
+
+[@@__reduce__; __steel_reduce__]
+let log_inv (l:log) (p: EP.bounded_u32 (U32.v l.len)) (bs: bytes_repr (U32.v l.len)) (s:repr) =
+    log_with_parsed_prefix_raw l.len l.arr l.pos l.ghost p bs s
+
+
+(* And dispose to unconditionally just drop the log and
+   return the underlying array *)
+assume
+val free (#s:repr)
+         (l:log)
+         (#p:Ghost.erased (EP.bounded_u32 (U32.v l.len)))
+         (#bs: bytes_repr (U32.v l.len))
+         (_:unit)
+  : SteelT unit
+    (log_inv l p bs s)
+    (fun _ -> A.varray (log_array l))
+
+
+let intro_read_next_provides_finished
+    (s:repr)
+    (r:read_result)
+    (l:log)
+  : Steel unit
+    (A.varray (log_array l))
+    (fun _ -> read_next_provides s l r)
+    (requires fun _ -> Failed? r)
+    (ensures fun _ _ _ -> True)
+  = AT.change_equal_slprop (A.varray (log_array l))
+                           (read_next_provides s l r);
+    AT.return ()
+
+val fail (#s:repr)
+         (l:log)
+         (#p:Ghost.erased (EP.bounded_u32 (U32.v l.len)))
+         (#bs: bytes_repr (U32.v l.len))
+         (pos:U32.t)
+  : Steel read_result
+    (log_inv l p bs s)
+    (fun r -> read_next_provides s l r)
+    (requires fun _ -> U32.v pos <= U32.v l.len)
+    (ensures fun _ r _ -> Failed? r /\ Failed?.pos r == pos)
+let fail #s l #p #bs pos
+  = free l ();
+    let res = Failed pos "" in
+    intro_read_next_provides_finished s res l;
+    AT.return res
+
+assume
+val read_pt (#a:Type) (#p:Perm.perm) (#v:Ghost.erased a) (r:R.ref a)
+  : Steel a (R.pts_to r p v) (fun x -> R.pts_to r p v)
+           (requires fun _ -> True)
+           (ensures fun _ x _ -> x == Ghost.reveal v)
+
+assume
+val extract_log_entry_from (len: U32.t)
+                           (buf: EP.larray U8.t len)
+                           (#bs: bytes_repr (U32.v len))
+                           (p: EP.bounded_u32 (U32.v len))
+  : Steel (either (T.vlog_entry & EP.bounded_u32 (U32.v len))
+                  (EP.bounded_u32 (U32.v len) & string))
+    (varray_pts_to_u8 buf bs)
+    (fun _ -> varray_pts_to_u8 buf bs)
+    (requires fun _ -> True)
+    (ensures fun h0 x h1 ->
+      (match x with
+       | Inl (e, p') ->
+         EP.valid_entry bs (U32.v p) (U32.v p') e
+       | Inr (p', _) ->
+         True))
+
+
+let st_extend_parsed_raw_util
+      (#len:nat) #o
+      (pos:EP.bounded_u32 len)
+      (s:bytes_repr len)
+      (r:repr)
+      (pos':EP.bounded_u32 len)
+      (e:T.vlog_entry)
+  : AT.SteelGhost unit o
+     (pure (parsed_raw_until pos s r))
+     (fun _ -> pure (parsed_raw_until pos' s (snoc_log r e)))
+     (requires fun _ ->
+       EP.valid_entry s (U32.v pos) (U32.v pos') e)
+     (ensures fun _ _ _ -> True)
+  = AT.sladmit()
+
+let read_next' #s l
+  = let h = AT.get () in
+    let pbs = elim_log_with_parsed_prefix l s in
+    let pos = read_pt l.pos in
+    if pos = l.len
+    then (
+      AT.sladmit();
+      AT.return Finished
+    )
+    else (
+      let eopt = extract_log_entry_from l.len l.arr pos in
+      match eopt with
+      | Inr (p, _) -> let r = fail l pos in AT.return r
+      | Inl (e, p') ->
+        st_extend_parsed_raw_util (fst pbs) _ s p' e;
+        AT.sladmit ();
+        AT.return (Failed p' "")
+    )
+
+    // if pos = l.len
+    // then (
+    // )
